roughing out LinkedJournal

Splinter/Paged/LinkedJournal.i.dfy
@@ -1,7 +1,7 @@
 // Copyright 2018-2021 VMware, Inc., Microsoft Inc., Carnegie Mellon University, ETH Zurich, and University of Washington
 // SPDX-License-Identifier: BSD-2-Clause
 
-include "PagedJournal.i.dfy"
+include "PagedJournalIfc.i.dfy"
 
 // The plan is something that refines to a TruncatedJournal.
 
@@ -9,12 +9,11 @@ module LinkedJournal {
   import opened Options
   import opened MsgHistoryMod
   import opened LSNMod
-
-  import PagedJournalIfc = PagedJournal // TODO(jonh): crack out ifc
+  import PagedJournalIfc
 
   type Pointer(==,!new)
 
-  datatype CacheView = CacheView(entries: map<Pointer, JournalRecord>) {
+  datatype CacheView = CacheView(entries: map<Pointer, JournalRecordType>) {
     function I(opointer: Option<Pointer>, used: set<Pointer>) : Option<PagedJournalIfc.JournalRecord>
       decreases entries.Keys - used
     {
@@ -32,12 +31,13 @@ module LinkedJournal {
     }
   }
 
-  datatype JournalRecord = JournalRecord(
+  // Kinda refines to PagedJournal.JournalRecord
+  datatype JournalRecordType = JournalRecordType(
     messageSeq: MsgHistory,
     priorRec: Option<Pointer>
   )
 
-  datatype TruncatedJournal = TruncatedJournal(
+  datatype TruncatedJournalType = TruncatedJournalType(
     boundaryLSN : LSN,  // exclusive: lsns <= boundaryLSN are discarded
     freshestRec: Option<Pointer>,
     cacheView: CacheView)
@@ -49,8 +49,73 @@ module LinkedJournal {
   }
 
   // implementation of JournalIfc obligations
-  function Mkfs() : (out:PersistentJournal)
+  function Mkfs() : (out:TruncatedJournalType)
   {
-    TruncatedJournal(0, None)
+    TruncatedJournalType(0, None, CacheView(map[]))
   }
+
+  predicate JR_WF(self: JournalRecordType)
+
+  function JR_I(self: JournalRecordType) : PagedJournalIfc.JournalRecord
+    requires JR_WF(self)
+
+  predicate TJ_WF(self: TruncatedJournalType)
+
+  function TJ_I(self: TruncatedJournalType) : (out: PagedJournalIfc.TruncatedJournal)
+    requires TJ_WF(self)
+    ensures out.WF()
+
+  function TJ_EmptyAt(lsn: LSN) : (out:TruncatedJournalType)
+    ensures TJ_WF(out)
+    ensures TJ_WF(out)
+    ensures TJ_I(out).I().EmptyHistory?
+    ensures TJ_I(out).boundaryLSN == lsn
+    ensures TJ_I(out).freshestRec.None?
+
+  function TJ_Mkfs() : (out:TruncatedJournalType)
+    ensures TJ_WF(out)
+    ensures TJ_I(out).I().EmptyHistory?
+  {
+    TJ_EmptyAt(0)
+  }
+
+  function TJ_DiscardOld(self: TruncatedJournalType, lsn: LSN) : (out:TruncatedJournalType)
+    requires TJ_WF(self)
+    requires TJ_I(self).I().CanDiscardTo(lsn)
+    ensures TJ_WF(out)
+    ensures TJ_I(out) == TJ_I(self).DiscardOld(lsn)
+
+  predicate TJ_CanDiscardRecentAtLine(self: TruncatedJournalType, i: nat)
+    requires TJ_WF(self)
+  {
+    && var receipt := TJ_I(self).BuildReceiptTJ();
+    && i < |receipt.lines|
+//    && assert receipt.lines[i].journalRec.messageSeq.MsgHistory? by { receipt.JournalRecsAllWF(); }
+  }
+
+  function TJ_DiscardRecent(self: TruncatedJournalType, i: nat) : (out:TruncatedJournalType)
+    requires TJ_WF(self)
+    requires TJ_CanDiscardRecentAtLine(self, i)
+    ensures TJ_WF(out)
+    ensures
+      var receipt := TJ_I(self).BuildReceiptTJ();
+      TJ_I(out) == PagedJournalIfc.TruncatedJournal(TJ_I(self).boundaryLSN, Some(receipt.lines[i].journalRec))
+
+  function TJ_AppendNewBoundary(self: TruncatedJournalType, msgs: MsgHistory) : (out:LSN)
+    requires TJ_WF(self)
+    requires msgs.MsgHistory?
+  {
+      if TJ_I(self).freshestRec.None?  // if tj is empty, its boundary is nonsense.
+      then msgs.seqStart
+      else TJ_I(self).boundaryLSN
+  }
+
+  function TJ_AppendRecord(self: TruncatedJournalType, msgs: MsgHistory) : (out:TruncatedJournalType)
+    requires TJ_WF(self)
+    requires msgs.MsgHistory?
+    requires TJ_I(self).Empty() || msgs.CanFollow(TJ_I(self).SeqEnd())
+    ensures TJ_WF(out)
+    ensures TJ_I(out) == PagedJournalIfc.TruncatedJournal(
+      TJ_AppendNewBoundary(self, msgs),
+      Some(PagedJournalIfc.JournalRecord(msgs, TJ_I(self).freshestRec)))
 }
